nola/examples/logic/adequacy.v
@@ -18,22 +18,22 @@ Definition nintpΣ : gFunctors :=
 #[export] Instance subG_nintpGpreS `{!subG nintpΣ Σ} : nintpGpreS Σ.
 Proof. solve_inG. Qed.
 
-(** Adequacy of [wp] over [nninv_wsatd] *)
+(** Adequacy of [wp] over [inv_wsatd] *)
 Lemma wp_n_adequacy `{!nintpGpreS Σ} {s e σ φ} :
-  (∀ `{!nintpGS Σ}, inv_heap_inv -∗ WP[nninv_wsatd] e @ s; ⊤ {{ v, ⌜φ v⌝ }}) →
+  (∀ `{!nintpGS Σ}, inv_heap_inv -∗ WP[inv_wsatd] e @ s; ⊤ {{ v, ⌜φ v⌝ }}) →
   adequate s e σ (λ v _, φ v).
 Proof.
   move=> towp. apply (heap_adequacy Σ HasNoLc)=> ?.
-  iMod ninv_wsat_alloc as (?) "?". iModIntro. iExists nninv_wsatd.
+  iMod inv_wsat_alloc as (?) "?". iModIntro. iExists inv_wsatd.
   iSplitL; [done|]. iApply (towp (NintpGS _ _ _ _ _)).
 Qed.
 
-(** Adequacy of [twp] over [nninv_wsatd] *)
+(** Adequacy of [twp] over [inv_wsatd] *)
 Lemma twp_n_adequacy `{!nintpGpreS Σ} {s e σ φ} :
-  (∀ `{!nintpGS Σ}, inv_heap_inv -∗ WP[nninv_wsatd] e @ s; ⊤ [{ v, ⌜φ v⌝ }]) →
+  (∀ `{!nintpGS Σ}, inv_heap_inv -∗ WP[inv_wsatd] e @ s; ⊤ [{ v, ⌜φ v⌝ }]) →
   sn erased_step ([e], σ).
 Proof.
   move=> totwp. apply (heap_total Σ s _ _ φ)=> ?.
-  iMod ninv_wsat_alloc as (?) "?". iModIntro. iExists nninv_wsatd.
+  iMod inv_wsat_alloc as (?) "?". iModIntro. iExists inv_wsatd.
   iSplitL; [done|]. iApply (totwp (NintpGS _ _ _ _ _)).
 Qed.
