nola/examples/logic/inv.v
@@ -7,44 +7,43 @@ Implicit Type P Q : nPropL (;ᵞ).
 Section lemmas.
   Context `{!nintpGS Σ}.
 
-  (** Access [nninv] *)
-  Lemma nninv_acc {N P E} : ↑N ⊆ E →
-    nninvd N P =[nninv_wsatd]{E,E∖↑N}=∗
-      ⟦ P ⟧ ∗ (⟦ P ⟧ =[nninv_wsatd]{E∖↑N,E}=∗ True).
+  (** Access [ninv] *)
+  Lemma ninv_acc {N P E} : ↑N ⊆ E →
+    ninvd N P =[inv_wsatd]{E,E∖↑N}=∗
+      ⟦ P ⟧ ∗ (⟦ P ⟧ =[inv_wsatd]{E∖↑N,E}=∗ True).
   Proof.
-    rewrite nninv_unseal. iIntros (NE) "#∝P". iDestruct nderiv_sound as "→".
+    rewrite ninv_unseal. iIntros (NE) "#∝P". iDestruct nderiv_sound as "→".
     iDestruct ("→" with "∝P") as "/={∝P}∝P". by iApply "∝P".
   Qed.
 
   Context `{!nderivy ih δ}.
 
-  (** Turn [ninv] into [nninv] *)
-  Lemma ninv_nninv (P : nPropS _) {N} :
-    ninv N (nInvd_u P) -∗ nninv (Σ:=Σ) δ N (↑ˡ P).
+  (** Turn [inv_tok] into [ninv] *)
+  Local Lemma inv_tok_ninv (P : nPropS _) {N} :
+    inv_tok N (nInvd_u P) -∗ ninv δ N (↑ˡ P).
   Proof.
-    rewrite nninv_unseal. iIntros "#NP !>". iApply (derivy_intro (δ:=δ))=>/=.
+    rewrite ninv_unseal. iIntros "#NP !>". iApply (derivy_intro (δ:=δ))=>/=.
     iIntros (?????). rewrite -nintpS_nintp_nlarge.
-    by iApply (ninv_acc with "NP").
+    by iApply (inv_tok_acc with "NP").
   Qed.
-
-  (** Allocate [nninv] *)
-  Lemma nninv_alloc_rec (P : nPropS _) {N} :
-    (nninv δ N (↑ˡ P) -∗ ⟦ P ⟧(δ)) =[nninv_wsat δ]=∗ nninv δ N (↑ˡ P).
+  (** Allocate [ninv] *)
+  Lemma ninv_alloc_rec (P : nPropS _) {N} :
+    (ninv δ N (↑ˡ P) -∗ ⟦ P ⟧(δ)) =[inv_wsat' δ]=∗ ninv δ N (↑ˡ P).
   Proof.
     iIntros "→P".
-    iMod (ninv_alloc_rec (P:=nInvd_u P) with "[→P]") as "NP".
-    - iIntros "/=NP". rewrite nintpS_nintp. iApply "→P". by iApply ninv_nninv.
-    - iModIntro. by iApply ninv_nninv.
+    iMod (inv_tok_alloc_rec (P:=nInvd_u P) with "[→P]") as "NP".
+    - iIntros "/=NP". rewrite nintpS_nintp. iApply "→P". by iApply inv_tok_ninv.
+    - iModIntro. by iApply inv_tok_ninv.
   Qed.
-  Lemma nninv_alloc (P : nPropS _) {N} :
-    ⟦ P ⟧(δ) =[nninv_wsat δ]=∗ nninv δ N (↑ˡ P).
-  Proof. iIntros "P". iApply (nninv_alloc_rec with "[P]"). by iIntros. Qed.
+  Lemma ninv_alloc (P : nPropS _) {N} :
+    ⟦ P ⟧(δ) =[inv_wsat' δ]=∗ ninv δ N (↑ˡ P).
+  Proof. iIntros "P". iApply (ninv_alloc_rec with "[P]"). by iIntros. Qed.
 
-  (** Transform [nninv] *)
-  Lemma nninv_convert {N P Q} :
-    □ ⸨ P ={∅}=∗ Q ∗ (Q ={∅}=∗ P) ⸩(δ) -∗ nninv δ N P -∗ nninv δ N Q.
+  (** Transform [ninv] *)
+  Lemma ninv_convert {N P Q} :
+    □ ⸨ P ={∅}=∗ Q ∗ (Q ={∅}=∗ P) ⸩(δ) -∗ ninv δ N P -∗ ninv δ N Q.
   Proof.
-    rewrite nninv_unseal. iIntros "#PQP #∝P !>".
+    rewrite ninv_unseal. iIntros "#PQP #∝P !>".
     iApply (derivy_map2 with "[] PQP ∝P")=>/=.
     iIntros (???) "/= {PQP}PQP {∝P}∝P". iIntros (? NE).
     iMod ("∝P" $! _ NE) as "[P P→]".
@@ -53,30 +52,30 @@ Section lemmas.
     iMod (fupd_mask_subseteq ∅) as "→E∖N"; [set_solver|].
     iMod ("QP" with "Q") as "P". iMod "→E∖N" as "_". iApply ("P→" with "P").
   Qed.
-  Lemma nninv_split {N P Q} :
-    nninv δ N (P ∗ Q) ⊢ nninv δ N P ∗ nninv δ N Q.
+  Lemma ninv_split {N P Q} :
+    ninv δ N (P ∗ Q) ⊢ ninv δ N P ∗ ninv δ N Q.
   Proof.
-    iIntros "#NPQ". iSplit; iApply (nninv_convert with "[] NPQ"); iModIntro;
+    iIntros "#NPQ". iSplit; iApply (ninv_convert with "[] NPQ"); iModIntro;
     iApply (derivy_intro (δ:=δ)); by iIntros (???) "/=[$$]!>$".
   Qed.
-  Lemma nninv_fupd {N P} :
-    nninv δ N (|={∅}=> P) ⊣⊢ nninv δ N P.
+  Lemma ninv_fupd {N P} :
+    ninv δ N (|={∅}=> P) ⊣⊢ ninv δ N P.
   Proof.
-    iSplit; iApply nninv_convert; iModIntro; iApply (derivy_intro (δ:=δ))=>/=;
+    iSplit; iApply ninv_convert; iModIntro; iApply (derivy_intro (δ:=δ))=>/=;
       iIntros (???); by [iIntros ">$!>$"|iIntros "$!>"; iSplitR; iIntros].
   Qed.
-  Lemma nninv_add {N P Q} :
-    □ ⸨ P ⸩(δ) -∗ nninv δ N Q -∗ nninv δ N (P ∗ Q).
+  Lemma ninv_add {N P Q} :
+    □ ⸨ P ⸩(δ) -∗ ninv δ N Q -∗ ninv δ N (P ∗ Q).
   Proof.
-    iIntros "#P". iApply nninv_convert. iModIntro.
+    iIntros "#P". iApply ninv_convert. iModIntro.
     iApply (derivy_map with "[] P"). by iIntros (???) "/=$$!>[_$]".
   Qed.
 
-  (** Combine [nninv]s *)
-  Lemma nninv_combine {N N' N'' P Q} : N ## N' → ↑N ∪ ↑N' ⊆@{coPset} ↑N'' →
-    nninv δ N P -∗ nninv δ N' Q -∗ nninv δ N'' (P ∗ Q).
+  (** Combine [ninv]s *)
+  Lemma ninv_combine {N N' N'' P Q} : N ## N' → ↑N ∪ ↑N' ⊆@{coPset} ↑N'' →
+    ninv δ N P -∗ ninv δ N' Q -∗ ninv δ N'' (P ∗ Q).
   Proof.
-    rewrite nninv_unseal. iIntros (??) "#NP #N'Q !>".
+    rewrite ninv_unseal. iIntros (??) "#NP #N'Q !>".
     iApply (derivy_map2 (δ:=δ) with "[] NP N'Q")=>/=.
     iIntros (???) "{NP}NP {N'Q}N'Q". iIntros (??).
     iMod ("NP" with "[%]") as "[$ P→]"; [set_solver|].
