nola/examples/logic/na_inv.v
@@ -7,13 +7,13 @@ Implicit Type P Q : nPropL (;ᵞ).
 Section lemmas.
   Context `{!nintpGS Σ}.
 
-  (** Access [na_nninv] *)
-  Lemma na_nninv_acc {p N P E F} : ↑N ⊆ E → ↑N ⊆ F →
-    na_nninvd p N P -∗ na_own p F =[nninv_wsatd]{E}=∗
+  (** Access [na_ninv] *)
+  Lemma na_ninv_acc {p N P E F} : ↑N ⊆ E → ↑N ⊆ F →
+    na_ninvd p N P -∗ na_own p F =[inv_wsatd]{E}=∗
       ⟦ P ⟧ ∗ na_own p (F∖↑N) ∗
-      (⟦ P ⟧ -∗ na_own p (F∖↑N) =[nninv_wsatd]{E}=∗ na_own p F).
+      (⟦ P ⟧ -∗ na_own p (F∖↑N) =[inv_wsatd]{E}=∗ na_own p F).
   Proof.
-    rewrite na_nninv_unseal. iIntros (NE NF) "#∝P F".
+    rewrite na_ninv_unseal. iIntros (NE NF) "#∝P F".
     iDestruct nderiv_sound as "→".
     iDestruct ("→" with "∝P") as "/={∝P}∝P".
     iApply ("∝P" $! _ _ NE NF with "F").
@@ -21,43 +21,43 @@ Section lemmas.
 
   Context `{!nderivy ih δ}.
 
-  (** Turn [na_ninv] into [na_nninv] *)
-  Lemma na_ninv_nninv (P : nPropS _) {i p N} : i ∈ (↑N:coPset) →
-    ninv N (nInvd_na p i P) -∗ na_nninv (Σ:=Σ) δ p N (↑ˡ P).
+  (** Turn [na_ninv] into [na_ninv] *)
+  Lemma na_ninv_ninv (P : nPropS _) {i p N} : i ∈ (↑N:coPset) →
+    inv_tok N (nInvd_na p i P) -∗ na_ninv (Σ:=Σ) δ p N (↑ˡ P).
   Proof.
-    rewrite na_nninv_unseal. iIntros (jN) "#NP !>".
+    rewrite na_ninv_unseal. iIntros (jN) "#NP !>".
     iApply (derivy_intro (δ:=δ))=>/=.
     iIntros (??? E F NE NF) "F". rewrite -nintpS_nintp_nlarge.
-    iMod (ninv_acc NE with "NP") as "/=[bd bd→]".
+    iMod (inv_tok_acc NE with "NP") as "/=[bd bd→]".
     iDestruct (na_body_acc with "bd F") as "(bd &$&$& P→)"; [done..|].
     iMod ("bd→" with "bd") as "_". iIntros "!> P F∖N".
-    iMod (ninv_acc NE with "NP") as "/=[bd bd→]".
+    iMod (inv_tok_acc NE with "NP") as "/=[bd bd→]".
     iDestruct ("P→" with "bd P F∖N") as "[bd $]".
     by iMod ("bd→" with "bd") as "_".
   Qed.
 
-  (** Allocate [na_nninv] *)
-  Lemma na_nninv_alloc_rec (P : nPropS _) {p N} :
-    (na_nninv δ p N (↑ˡ P) -∗ ⟦ P ⟧(δ)) =[nninv_wsat δ]=∗
-      na_nninv δ p N (↑ˡ P).
+  (** Allocate [na_ninv] *)
+  Lemma na_ninv_alloc_rec (P : nPropS _) {p N} :
+    (na_ninv δ p N (↑ˡ P) -∗ ⟦ P ⟧(δ)) =[inv_wsat' δ]=∗
+      na_ninv δ p N (↑ˡ P).
   Proof.
     iIntros "→P". iMod na_lock_alloc as (i) "[% lock]".
-    iMod (ninv_alloc_rec (P:=nInvd_na p i P) with "[→P lock]") as "NP".
+    iMod (inv_tok_alloc_rec (P:=nInvd_na p i P) with "[→P lock]") as "NP".
     - iIntros "/=NP". iLeft. iFrame "lock". rewrite nintpS_nintp.
-      iApply "→P". by iApply na_ninv_nninv.
-    - iModIntro. by iApply na_ninv_nninv.
+      iApply "→P". by iApply na_ninv_ninv.
+    - iModIntro. by iApply na_ninv_ninv.
   Qed.
-  Lemma na_nninv_alloc (P : nPropS _) {p N} :
-    ⟦ P ⟧(δ) =[nninv_wsat δ]=∗ na_nninv δ p N (↑ˡ P).
+  Lemma na_ninv_alloc (P : nPropS _) {p N} :
+    ⟦ P ⟧(δ) =[inv_wsat' δ]=∗ na_ninv δ p N (↑ˡ P).
   Proof.
-    iIntros "P". iApply (na_nninv_alloc_rec with "[P]"). by iIntros.
+    iIntros "P". iApply (na_ninv_alloc_rec with "[P]"). by iIntros.
   Qed.
 
-  (** Transform [na_nninv] *)
-  Lemma na_nninv_convert {p N P Q} :
-    □ ⸨ P ={∅}=∗ Q ∗ (Q ={∅}=∗ P) ⸩(δ) -∗ na_nninv δ p N P -∗ na_nninv δ p N Q.
+  (** Transform [na_ninv] *)
+  Lemma na_ninv_convert {p N P Q} :
+    □ ⸨ P ={∅}=∗ Q ∗ (Q ={∅}=∗ P) ⸩(δ) -∗ na_ninv δ p N P -∗ na_ninv δ p N Q.
   Proof.
-    rewrite na_nninv_unseal. iIntros "#PQP #∝P !>".
+    rewrite na_ninv_unseal. iIntros "#PQP #∝P !>".
     iApply (derivy_map2 with "[] PQP ∝P")=>/=.
     iIntros (???) "/= {PQP}PQP {∝P}∝P". iIntros (E F NE NF) "F".
     iMod ("∝P" $! E F NE NF with "F") as "(P &$& P→)".
@@ -66,31 +66,31 @@ Section lemmas.
     iMod (fupd_mask_subseteq ∅) as "→E∖N"; [set_solver|].
     iMod ("QP" with "Q") as "P". iMod "→E∖N" as "_". iApply ("P→" with "P").
   Qed.
-  Lemma na_nninv_split {p N P Q} :
-    na_nninv δ p N (P ∗ Q) ⊢ na_nninv δ p N P ∗ na_nninv δ p N Q.
+  Lemma na_ninv_split {p N P Q} :
+    na_ninv δ p N (P ∗ Q) ⊢ na_ninv δ p N P ∗ na_ninv δ p N Q.
   Proof.
-    iIntros "#NPQ". iSplit; iApply (na_nninv_convert with "[] NPQ"); iModIntro;
+    iIntros "#NPQ". iSplit; iApply (na_ninv_convert with "[] NPQ"); iModIntro;
     iApply (derivy_intro (δ:=δ)); by iIntros (???) "/=[$$]!>$".
   Qed.
-  Lemma na_nninv_fupd {p N P} :
-    na_nninv δ p N (|={∅}=> P) ⊣⊢ na_nninv δ p N P.
+  Lemma na_ninv_fupd {p N P} :
+    na_ninv δ p N (|={∅}=> P) ⊣⊢ na_ninv δ p N P.
   Proof.
-    iSplit; iApply na_nninv_convert; iModIntro;
+    iSplit; iApply na_ninv_convert; iModIntro;
       iApply (derivy_intro (δ:=δ))=>/=; iIntros (???);
       by [iIntros ">$!>$"|iIntros "$!>"; iSplitR; iIntros].
   Qed.
-  Lemma na_nninv_add {p N P Q} :
-    □ ⸨ P ⸩(δ) -∗ na_nninv δ p N Q -∗ na_nninv δ p N (P ∗ Q).
+  Lemma na_ninv_add {p N P Q} :
+    □ ⸨ P ⸩(δ) -∗ na_ninv δ p N Q -∗ na_ninv δ p N (P ∗ Q).
   Proof.
-    iIntros "#P". iApply na_nninv_convert. iModIntro.
+    iIntros "#P". iApply na_ninv_convert. iModIntro.
     iApply (derivy_map with "[] P"). by iIntros (???) "/=$$!>[_$]".
   Qed.
 
-  (** Combine [na_nninv]s *)
-  Lemma nninv_combine {p N N' N'' P Q} : N ## N' → ↑N ∪ ↑N' ⊆@{coPset} ↑N'' →
-    na_nninv δ p N P -∗ na_nninv δ p N' Q -∗ na_nninv δ p N'' (P ∗ Q).
+  (** Combine [na_ninv]s *)
+  Lemma ninv_combine {p N N' N'' P Q} : N ## N' → ↑N ∪ ↑N' ⊆@{coPset} ↑N'' →
+    na_ninv δ p N P -∗ na_ninv δ p N' Q -∗ na_ninv δ p N'' (P ∗ Q).
   Proof.
-    rewrite na_nninv_unseal. iIntros (??) "#NP #N'Q !>".
+    rewrite na_ninv_unseal. iIntros (??) "#NP #N'Q !>".
     iApply (derivy_map2 (δ:=δ) with "[] NP N'Q")=>/=.
     iIntros (???) "{NP}NP {N'Q}N'Q". iIntros (? F ??) "F".
     iMod ("NP" with "[%] [%] F") as "($& F∖N & P→)"; [set_solver..|].
